reduction_directedHamiltonianCircuit_to_hamiltonianCircuit/left_lemma_working_file.dfy
@@ -1,0 +1,124 @@
+include "reduction_hamiltonian_definitions.dfy"
+include "reduction_hamiltonian_rFunction.dfy"
+include "permutation_property.dfy"
+include "reduction_hamiltonian_rCompletness.dfy"
+
+module LeftLemma
+{
+    import opened Definitions
+    import opened ReductionFunction
+    import opened PermutationProperty
+    import opened ReductionCompletness
+
+    lemma reduction_lemma_left(g: Graph)
+        requires validGraph(g)
+        requires undirectedHamiltonianCircuit(directed_to_undirected_graph(g))
+        ensures directedHamiltonianCircuit(g)
+    {
+
+    }
+
+    function rSeq(s: seq<int>): seq<int>
+    {
+        if |s| == 0 then
+            []
+        else
+            rSeq(s[1..]) + [s[0]]
+    }
+
+    lemma circuit_reverse_property_lemma(g: Graph, c: seq<nat>)
+        requires validUndirectedGraph(g)
+        requires |g|>2
+        requires isUndirectedHamiltonianCircuit(g, c)
+        ensures isUndirectedHamiltonianCircuit(g, c)
+    {}
+
+    ghost function cicle_sequence(s: seq<nat>, i: int): seq<nat>
+        requires 0<=i<|s|
+    {
+        s[i..|s|] + s[0..i]
+    }
+
+    lemma circuit_circular_property_lemma(g: Graph, c: seq<nat>)
+        requires validUndirectedGraph(g)
+        requires |g|>2
+        requires isUndirectedHamiltonianCircuit(g, c)
+        ensures forall i :: 0<=i<|c| ==> isUndirectedHamiltonianCircuit(g, cicle_sequence(c, i))
+    {}
+
+    ghost predicate in_out_circuit(g: Graph, uc: seq<nat>)
+        requires validUndirectedGraph(g)
+        requires |g|>2 && |g|%3==0
+        requires in_out_graph(g)
+        // requires isUndirectedHamiltonianCircuit(g, uc)
+    {
+        isUndirectedHamiltonianCircuit(g, uc)
+        &&
+        forall i :: 0<i<|uc|-1 ==>
+        (
+            (0<=uc[i]<|g|/3 ==>  //case og node
+            (
+                uc[i-1]==uc[i]+(|g|/3)*2  //before: in
+                &&
+                uc[i+1]==uc[i]+|g|/3    //next: out
+            ))
+            &&
+            (|g|/3<=uc[i]<(|g|/3)*2 ==>  //case out node
+            (
+                uc[i-1]==uc[i]-|g|/3   //before: og
+                &&
+                (|g|/3)*2<=uc[i+1]<|g|   //next: in (range)
+            ))
+            &&
+            ((|g|/3)*2<=uc[i]<|g| ==>  //case in node
+            (
+                |g|/3<=uc[i-1]<(|g|/3)*2   //before: out (range)
+                &&
+                uc[i+1]==uc[i]-(|g|/3)*2    //next: og
+            ))
+        )
+    }
+
+    lemma in_out_circuit_lemma(g: Graph, c: seq<nat>)
+        requires validUndirectedGraph(g)
+        requires |g|>2 && |g|%3==0
+        requires isUndirectedHamiltonianCircuit(g, c)
+        requires in_out_graph(g)
+        ensures in_out_circuit(g, c)
+    {
+        
+    }
+
+    //starts with in_node -> og_node -> out_node ...and so on...
+    ghost predicate in_out_circuit_std(g: Graph, uc: seq<nat>)
+        requires validUndirectedGraph(g)
+        requires |g|>2 && |g|%3==0
+        requires in_out_graph(g)
+        // requires isUndirectedHamiltonianCircuit(g, uc)
+        ensures in_out_circuit_std(g, uc) ==> in_out_circuit(g, uc)
+    {
+        isUndirectedHamiltonianCircuit(g, uc)
+        &&
+        forall i :: 0<=i<|uc| && i%3==1 ==>
+        (
+            0<=uc[i]<|g|/3  //this: og_node
+            &&
+            uc[i-1]==uc[i]+(|g|/3)*2    //prev: *in_node
+            &&
+            uc[i+1]==uc[i]+|g|/3    //next: *out_node
+        )
+    }
+
+    ghost function standarize_in_out_circuit(g: Graph, uc: seq<nat>): seq<nat>
+        requires validUndirectedGraph(g)
+        requires |g|>2 && |g|%3==0
+        requires in_out_graph(g)
+        requires in_out_circuit(g, uc)
+        // ensures in_out_circuit_std(g, standarize_in_out_circuit(g, uc))
+    {
+        if |g|/3<=uc[0]<(|g|/3)*2 then cicle_sequence(uc, 0)    //0: out -> put [0] at the end
+        else if 0<=uc[0]<|g|/3 then cicle_sequence(uc, 1)   //0: og -> put [0,1] at the end
+        else uc //0: in -> already std
+    }
+
+}
