reduction_directedHamiltonianCircuit_to_hamiltonianCircuit/reduction_hamiltonian_definitions.dfy
@@ -35,12 +35,11 @@ module Definitions
     ghost predicate directedHamiltonianCircuit(g: Graph)
         requires validGraph(g)
     {
-        |g|>2 && exists hc :: isDirectedHamiltonianCircuit(g, hc)
+        exists hc :: isDirectedHamiltonianCircuit(g, hc)
     }
 
     ghost predicate isDirectedHamiltonianCircuit(g: Graph, circuit: seq<nat>)
         requires validGraph(g)
-        requires |g|>2
         // ensures forall i :: 0<i<|g| ==> g[circuit[i-1]][circuit[i]]
     {
         hamiltonianCircuitPartialCorrectness(g, circuit) && isDirectedHamiltonianCircuit3(g, circuit)
@@ -74,9 +73,9 @@ module Definitions
 
     ghost predicate isDirectedHamiltonianCircuit3(g: Graph, circuit: seq<nat>)
         requires validGraph(g)
-        requires |g|>2
         requires hamiltonianCircuitPartialCorrectness(g, circuit)
     {
+        |g|>0 &&
         (forall i :: 0<i<|g| ==> g[circuit[i-1]][circuit[i]]) && (g[circuit[|g|-1]][circuit[0]])
     }
 
@@ -162,12 +161,11 @@ module Definitions
     ghost predicate undirectedHamiltonianCircuit(g: Graph)
         requires validUndirectedGraph(g)
     {
-        |g|>2 && exists hc :: isUndirectedHamiltonianCircuit(g, hc)
+        exists hc :: isUndirectedHamiltonianCircuit(g, hc)
     }
 
     ghost predicate isUndirectedHamiltonianCircuit(g: Graph, circuit: seq<nat>)
         requires validUndirectedGraph(g)
-        requires |g|>2
     {
         hamiltonianCircuitPartialCorrectness(g, circuit) && isUndirectedHamiltonianCircuit3(g, circuit)
     }
@@ -185,8 +183,8 @@ module Definitions
     ghost predicate isUndirectedHamiltonianCircuit3(g: Graph, circuit: seq<nat>)
         requires validUndirectedGraph(g)
         requires hamiltonianCircuitPartialCorrectness(g, circuit)
-        requires |g|>2
     {
+        |g|>0 &&
         (forall i :: 0<i<|g| ==> (g[circuit[i-1]][circuit[i]] || g[circuit[i]][circuit[i-1]])) &&  (g[circuit[|g|-1]][circuit[0]] || g[circuit[0]][circuit[|g|-1]])
     }
 
